Magic.v
@@ -1,0 +1,8 @@
+Unset Guard Checking.
+
+Fixpoint magic (x : nat) : False := magic x.
+
+Goal False.
+  apply magic. exact 0.
+Qed.
+
