ShadowInterpList.v
@@ -1,0 +1,197 @@
+From Coq Require Import Arith String List.
+Import ListNotations.
+
+Local Open Scope string_scope.
+
+Inductive tm :=
+  | Var (x : string)
+  | Fn (x : string) (e : tm)
+  | App (f a : tm)
+  | Link (m e : tm)
+  | Mt
+  | Bind (x : string) (v m : tm)
+.
+
+Inductive env :=
+  | Env (β : list (string * val)) (s : option shadow)
+
+with val :=
+  | Clos (x : string) (k : list val) (σ : env)
+  | Mod (σ : env)
+  | Shadow_val (s : shadow)
+
+with shadow :=
+  | Init
+  | Read (s : shadow) (x : string)
+  | Call (s : shadow) (v : val)
+.
+
+Local Notation "'⟨' 'λ' x k σ '⟩'" := (Clos x k σ) (at level 60, right associativity, only printing).
+Local Notation "'⟨' σ '⟩'" := (Mod σ) (at level 60, right associativity, only printing).
+Local Notation "'⟨' s '⟩'" := (Shadow_val s) (at level 60, right associativity, only printing).
+Local Notation "'⟪' β  s '⟫'" := (Env β (Some s)) (at level 60, right associativity, only printing).
+Local Notation "'⟪' β  • '⟫'" := (Env β None) (at level 60, right associativity, only printing).
+
+Definition ω := Fn "x" (App (Var "x") (Var "x")).
+Definition ι := Fn "x" (Var "x").
+Definition α := Fn "f" (Fn "x" (App (Var "f") (Var "x"))).
+
+Definition upd_env (σ : env) (x : string) (v : val) :=
+  match σ with
+  | Env β s => Env ((x, v) :: β) s
+  end.
+
+Definition app_env β σ :=
+  match σ with
+  | Env β' s => Env (β ++ β') s
+  end.
+
+Fixpoint read_list (β : list (string * val)) (x : string) :=
+  match β with
+  | [] => None
+  | (x', v) :: β' =>
+    if x =? x' then Some v else read_list β' x
+  end.
+
+Definition read_env (σ : env) (x : string) :=
+  match σ with
+  | Env β s =>
+    match read_list β x with
+    | Some v => Some v
+    | None =>
+      match s with
+      | None => None
+      | Some s => Some (Shadow_val (Read s x))
+      end
+    end
+  end.
+
+Definition eval (link : env -> val -> list val) :=
+  fix eval (e : tm) : list val :=
+  match e with
+  | Var x => [Shadow_val (Read Init x)]
+  | Fn x M => [Clos x (eval M) (Env [] (Some Init))]
+  | App M N =>
+    let foldM acc fn :=
+      let foldN acc' arg :=
+        match fn with
+        | Clos x B σ =>
+          flat_map (link (upd_env σ x arg)) B ++ acc'
+        | Shadow_val fn =>
+          Shadow_val (Call fn arg) :: acc'
+        | Mod _ => acc'
+        end
+      in fold_left foldN (eval N) acc
+    in fold_left foldM (eval M) []
+  | Link M N =>
+    let foldM acc m :=
+      let foldN acc' cli :=
+        match m with
+        | Mod σ =>
+          link σ cli ++ acc'
+        | Shadow_val m =>
+          link (Env [] (Some m)) cli ++ acc'
+        | Clos _ _ _ => acc'
+        end
+      in fold_left foldN (eval N) acc
+    in fold_left foldM (eval M) []
+  | Mt => [Mod (Env [] None)]
+  | Bind x M N =>
+    let foldM acc v :=
+      let foldN acc' m :=
+        let foldL acc'' m' :=
+          match m' with
+          | Mod σ => Mod (upd_env σ x v) :: acc''
+          | Shadow_val s => Mod (Env [(x, v)] (Some s)) :: acc''
+          | Clos _ _ _ => acc''
+          end
+        in fold_left foldL (link (Env [(x, v)] (Some Init)) m) acc'
+      in fold_left foldN (eval N) acc
+    in fold_left foldM (eval M) []
+  end%list.
+
+(* linking, up to n steps *)
+Fixpoint link (n : nat) (σ : env) : val -> list val :=
+  match n with 0 => (fun _ => []) | S n =>
+  fix link_val v : list val :=
+    match v with
+    | Clos x k σ' => map (Clos x k) (link_env σ')
+    | Mod σ' => map Mod (link_env σ')
+    | Shadow_val s => link_shadow s
+    end
+  with link_env σ' : list env :=
+    let fix link_list β :=
+      match β with
+      | [] => [[]] 
+      | (x, v) :: β =>
+        let foldv acc v :=
+          let foldβ acc' β := ((x, v) :: β) :: acc'
+          in fold_left foldβ (link_list β) acc
+        in fold_left foldv (link_val v) []
+      end
+    in match σ' with
+    | Env β None => map (fun β => Env β None) (link_list β)
+    | Env β (Some s) =>
+      let folds acc s :=
+        let foldβ acc' β :=
+          match s with
+          | Mod σ => app_env β σ :: acc'
+          | Shadow_val s => Env β (Some s) :: acc'
+          | Clos _ _ _ => acc'
+          end
+        in fold_left foldβ (link_list β) acc
+      in fold_left folds (link_shadow s) []
+    end
+  with link_shadow s : list val :=
+    match s with
+    | Init => [Mod σ]
+    | Read s x =>
+      let folds acc s :=
+        match s with
+        | Mod σ =>
+          match read_env σ x with
+          | None => acc
+          | Some v => v :: acc
+          end
+        | Shadow_val s => Shadow_val (Read s x) :: acc
+        | Clos _ _ _ => acc
+        end
+      in fold_left folds (link_shadow s) []
+    | Call s v =>
+      let folds acc s :=
+        let foldv acc' v :=
+          match s with
+          | Clos x k σ =>
+            flat_map (link n (upd_env σ x v)) k ++ acc'
+          | Shadow_val s =>
+            Shadow_val (Call s v) :: acc'
+          | Mod _ => acc'
+          end
+        in fold_left foldv (link_val v) acc
+      in fold_left folds (link_shadow s) []
+    end
+  for link_val
+  end%list.
+
+Definition interp n := eval (link n).
+
+Local Coercion Shadow_val : shadow >-> val.
+Local Coercion Mod : env >-> val.
+Compute interp 1 ω.
+Compute interp 100 (App ω ω).
+Compute interp 1 (App ι ι).
+Definition test_module := Bind "app" α (Bind "id" ι Mt).
+Definition open1 := App (Var "id") (Var "id").
+Definition open2 := App (Var "app") (Var "id").
+Definition compute_in_fun1 := Fn "x" (App (App ι ι) (Var "x")).
+Definition compute_in_fun2 := Fn "x" (App ι (App ι (Var "x"))).
+Compute interp 2 (Link test_module open1).
+Compute interp 2 (Link test_module open2).
+Compute interp 1 compute_in_fun1.
+Compute interp 1 compute_in_fun2.
+
+Definition bomb := Bind "w" ω Mt.
+Definition bomber := Bind "div" (App (Var "w") (Var "w")) Mt.
+Compute interp 1 (Link bomb (Link bomber Mt)).
+Compute interp 100 (Link (Link bomb bomber) Mt).
+
