README.md
@@ -1,5 +1,14 @@
-# CPS Playground
+# Coq Interpreter Playground
+
+Multiple examples of interpreters (with fuel), written in Coq.
+
+## CPS transformer([CPS.v](CPS.v))
 
 A CPS transformer and evaluator of a functional language featuring `raise` and `handle` operations.
 
-Written in Coq.
+## λ-calculus with modules
+
+- Without recursion, using options ([ShadowInterpOption.v](ShadowInterpOption.v))
+- Without recursion, using lists ([ShadowInterpList.v](ShadowInterpList.v))
+- With recursion, using lists ([ShadowInterpRec.v](ShadowInterpRec.v))
+
